

To prove

$$\frac{\partial C}{\partial b_j^l} = \delta_j^l$$

$$\frac{\partial C}{\partial b_j^l} = \frac{\partial C}{\partial z_j^l} \times \frac{\partial z_j^l}{\partial b_j^l}$$

$$\therefore \frac{\partial C}{\partial z_j^l} = \delta_j^l$$

$$\frac{\partial C}{\partial z_j^l} \frac{\partial z_j^l}{\partial b_j^l} = \delta_j^l$$

if this true $\delta_j^l \times \frac{\partial z_j^l}{\partial b_j^l} = \delta_j^l$

This must be true $\frac{\partial z_j^l}{\partial b_j^l} = 1$ $z_j^l = w_{jk}^l a_k^{l-1} + b_j^l$

$$\frac{\partial (w_{jk}^l a_k^{l-1} + b_j^l)}{\partial b_j^l} = \frac{\partial (w_{jk}^l a_k^{l-1})}{\partial b_j^l} + \frac{\partial b_j^l}{\partial b_j^l}$$

$$= 0 + 1 = 1$$

Here

hence proved.

$$\boxed{\frac{\partial C}{\partial b_j^l} = \delta_j^l}$$

$$\textcircled{9} \frac{\partial C}{\partial w_{jk}^l} = a_k^{l-1} \delta_j^l$$

$$\frac{\partial C}{\partial z_j^l} \frac{\partial z_j^l}{\partial w_{jk}^l} = a_k^{l-1} \delta_j^l \quad \frac{\partial C}{\partial z_j^l} = \delta_j^l$$

so To prove this we have to prove that

$$\frac{\partial z_j^l}{\partial w_{jk}^l} = a_k^{l-1}$$

$$\frac{\partial (w_{jk}^l \cdot a_k^{l-1} + b_j^l)}{\partial w_{jk}^l}$$

$$= \frac{\partial (w_{jk}^l a_k^{l-1})}{\partial w_{jk}^l} + \frac{\partial (b_j^l)}{\partial w_{jk}^l}$$

$$= a_k^{l-1} + 0 = a_k^{l-1}$$

Hence proved.

③

$$BP_1 \Rightarrow \frac{\partial C}{\partial z_j^l} = \delta_j^l$$

$$\delta_j^L = \frac{\partial C}{\partial a_j^L} \cdot \frac{\partial a_j^L}{\partial z_j^L}$$

$$= \frac{\partial C}{\partial a_j^L} \cdot \frac{\partial (f(z_j^L))}{\partial z_j^L}$$

$$\boxed{\delta_j^L = \frac{\partial C}{\partial a_j^L} \cdot f'(z_j^L)}$$

16y

BP₂ ⇒

$$\delta^L = ((w^{L+1})^T \delta^{L+1}) \odot \sigma'(z^L)$$

BP₃ ⇒

$$\frac{\partial C}{\partial b_j^l} = \frac{\partial C}{\partial z_j^l} \cdot \frac{\partial z_j^l}{\partial b_j^l}$$

$$= \frac{\partial C}{\partial z_j^l} = \delta_j^l //$$

BP₄ ⇒

$$\frac{\partial C}{\partial w_{jk}^l} = \frac{\partial C}{\partial z_j^l} \cdot \frac{\partial z_j^l}{\partial w_{jk}^l}$$

$$\frac{\partial C}{\partial w_{jk}^l} = \delta_j^l \cdot \frac{\partial (w_{jk}^{l+1} a_j^l + b_k^{l+1})}{\partial w_{jk}^l} = \delta_j^l \cdot a_k^{l+1} //$$

③

$$BP_1 \Rightarrow \frac{\partial C}{\partial z_j^l} = \delta_j^l$$

$$\begin{aligned} \delta_j^L &= \frac{\partial C}{\partial a_j^L} \cdot \frac{\partial a_j^L}{\partial z_j^L} \\ &= \frac{\partial C}{\partial a_j^L} \cdot \frac{\partial (f(z_j^L))}{\partial z_j^L} \end{aligned}$$

$$\boxed{\delta_j^L = \frac{\partial C}{\partial a_j^L} \cdot f'(z_j^L)}$$

by

BP₂ ⇒

$$\delta^L = ((\omega^{L+1})^T \delta^{L+1}) \odot \sigma'(z^L)$$

BP₃ ⇒

$$\begin{aligned} \frac{\partial C}{\partial b_j^l} &= \frac{\partial C}{\partial z_j^l} \cdot \frac{\partial z_j^l}{\partial b_j^l} \\ &= \frac{\partial C}{\partial z_j^l} = \delta_j^l \quad // \end{aligned}$$

BP₄ ⇒

$$\frac{\partial C}{\partial \omega_{jk}^l} = \frac{\partial C}{\partial z_j^l} \cdot \frac{\partial z_j^l}{\partial \omega_{jk}^l}$$

$$\frac{\partial C}{\partial \omega_{jk}^l} = \delta_j^l \cdot \frac{\partial (\omega_{jk}^{l-1} a_k^{l-1} + b_j^l)}{\partial \omega_{jk}^l} = \delta_j^l \cdot a_k^{l-1} \quad //$$

④ ab $\sigma(z) = z \Rightarrow f(z) = z$

BP₁ $\Rightarrow \delta_j^L = \frac{\partial C}{\partial a_j^L} f'(z_j^L)$

$$\delta_j^L = \frac{\partial C}{\partial a_j^L} \cdot \frac{\partial f(z)}{\partial z}$$

$$= \frac{\partial C}{\partial a} \cdot \frac{\partial z}{\partial z} = \frac{\partial C}{\partial a} \cdot 1$$

$$\delta_j^L = \frac{\partial C}{\partial a_j^L}$$

BP₂ $\Rightarrow \delta_j^l = \frac{\partial C}{\partial z_j^l} = \sum_k \frac{\partial C}{\partial z_k^{l+1}} \frac{\partial z_k^{l+1}}{\partial z_j^l}$

from previous eqn

$$\delta_j^l = \sum_k \left(w_{kj}^{l+1} \cdot \frac{\partial (z_j^l)}{\partial (z_k^{l+1})} \cdot \frac{\partial C}{\partial z_k^{l+1}} \right) \delta_k^{l+1}$$

$$= \sum_k \delta_k^{l+1} w_{kj}^{l+1} \frac{\partial (z_j^l)}{\partial (z_k^{l+1})}$$

$$= \sum_k \delta_k^{l+1} w_{kj}^{l+1} \cdot 1$$

2. σ

$$\frac{\partial(\sigma(z))}{\partial(z)} = \sigma'(z) \text{ gives the}$$

derivative of the neuron

so we can know that if it is near the predicted output.

so the error value doesn't know about the actual ~~gradient~~ gradient (from slope of σ)

BP₃ \Rightarrow

$$\frac{\partial C}{\partial b_j^1} = \delta_j^1$$

BP₄ \Rightarrow

$$\frac{\partial C}{\partial w_{jk}^1} = a_k^{1-1} \delta_j^1$$

In BP₃ and BP₄ The ~~value~~ formula doesn't change but the actual value is calculated from BP₁ and BP₂ so it is also affected in the value